Source/DafnyRuntime/DafnyRuntimeDafny/src/atomicBox.dfy
@@ -1,51 +1,17 @@
 
-include "array.dfy"
-include "frames.dfy"
-
-module {:options "/functionSyntax:4"} AtomicBoxes {
-  import opened Arrays
-  import opened Frames
-
-  trait {:termination false} AtomicBox<T> extends Validatable {
-
-    ghost predicate Valid()
-      reads this, Repr
-      ensures Valid() ==> Repr == {}
+module AtomicBoxes {
+  class {:extern} AtomicBox<T> {
 
     ghost const inv: T -> bool
 
-    method {:extern} Put(t: T)
+    static method Make(ghost inv: T -> bool, t: T) returns (ret: AtomicBox<T>)
       requires inv(t)
+      ensures ret.inv == inv
 
-    method {:extern} Get() returns (t: T)
+    method Get() returns (t: T)
       ensures inv(t)
+
+    method Put(t: T)
+      requires inv(t)
   }
-
-  // Feasibility implementation
-  // DO NOT USE THIS as it is not guaranteed to be atomic!
-  //
-  // Using Array<T> as an arbitrary type that needs an invariant.
-  // class DafnyNotActuallyAtomicBox<T> extends AtomicBox<Array<T>> {
-
-  //   var value: Array<T>
-
-  //   constructor(inv: Array<T> -> bool, value: Array<T>) 
-  //     requires inv(value)
-  //   {
-  //     this.inv := inv;
-  //     this.value := value;
-  //   }
-
-  //   method Put(value: Array<T>)
-  //     requires inv(value)
-  //   {
-  //     this.value := value;
-  //   }
-
-  //   method Get() returns (value: Array<T>)
-  //     ensures inv(value)
-  //   {
-  //     return this.value;
-  //   }
-  // }
 }
